theories/Syntax/Patterns.v
@@ -34,6 +34,7 @@ From Katamaran Require Import
 
 Import ctx.notations.
 Import env.notations.
+Import SigTNotations.
 
 Module Type PatternsOn (Import TY : Types).
 
@@ -223,6 +224,217 @@ Module Type PatternsOn (Import TY : Types).
       - destruct env.snocView, env.snocView.
         destruct (env.nilView E).
         now rewrite bv.appView_app.
+    Qed.
+
+    (* A [PatternShape] describes the different pattern matching possibilities.
+       Not every type can be matched on, and some types can be matched on in
+       different ways, e.g. bitvectors. The [PatternShape], as opposed to the
+       [PatternCase] below, is a value that is provided by the user in the
+       program and therefore includes all the names ((program or logic
+       variables) for all alternatives of that match. For example
+       [pat_shape_sum] contains the names [x] and [y] for the [inl] and [inr]
+       cases. *)
+    Inductive PatternShape : Ty -> Set :=
+    | pat_shape_bool                                        : PatternShape ty.bool
+    | pat_shape_list σ (x y : N)                            : PatternShape (ty.list σ)
+    | pat_shape_prod σ τ (x y : N)                          : PatternShape (ty.prod σ τ)
+    | pat_shape_sum σ τ (x y : N)                           : PatternShape (ty.sum σ τ)
+    | pat_shape_unit                                        : PatternShape ty.unit
+    | pat_shape_enum E                                      : PatternShape (ty.enum E)
+    | pat_shape_bvec_split m n (x y : N)                    : PatternShape (ty.bvec (m+n))
+    | pat_shape_bvec_exhaustive m                           : PatternShape (ty.bvec m)
+    | pat_shape_tuple σs Δ (p : TuplePat σs Δ)              : PatternShape (ty.tuple σs)
+    | pat_shape_union U (x : N)                             : PatternShape (ty.union U)
+    | pat_shape_record R Δ (p : RecordPat (recordf_ty R) Δ) : PatternShape (ty.record R).
+
+    (* This describes the different cases/alternatives for a single pattern
+       match of a particular shape. It can be seen as a representation of the
+       arity of a match. *)
+    Definition PatternCase {σ} (pat : PatternShape σ) : Set :=
+      match pat with
+      | pat_shape_bool               => bool
+      | pat_shape_list σ x y         => bool
+      | pat_shape_prod σ τ x y       => unit
+      | pat_shape_sum σ τ x y        => bool
+      | pat_shape_unit               => unit
+      | pat_shape_enum E             => enumt E
+      | pat_shape_bvec_split m n x y => unit
+      | pat_shape_bvec_exhaustive m  => bv m
+      | pat_shape_tuple σs Δ p       => unit
+      | pat_shape_union U x          => unionk U
+      | pat_shape_record R Δ p       => unit
+      end.
+
+    #[export] Instance EqDec_PatternCase {σ} (pat : PatternShape σ) :
+      Classes.EqDec (PatternCase pat) :=
+      ltac:(destruct pat; cbn [PatternCase];
+            auto with typeclass_instances).
+
+    #[export] Instance Finite_PatternCase {σ} (pat : PatternShape σ) :
+      finite.Finite (PatternCase pat) :=
+      ltac:(destruct pat; cbn [PatternCase EqDec_PatternCase];
+            auto with typeclass_instances).
+
+    (* For each [PatternShape] and each [PatternCase] for that shape, calculate
+       the context that represents the variables bound in that case. *)
+    Definition PatternCaseCtx {σ} {p : PatternShape σ} : PatternCase p -> NCtx N Ty :=
+      match p with
+      | pat_shape_bool               => fun _ => [ctx]
+      | pat_shape_list σ x y         => fun b => if b then [ctx] else [x∷σ; y∷ty.list σ]
+      | pat_shape_prod σ τ x y       => fun _ => [x∷σ; y∷τ]
+      | pat_shape_sum σ τ x y        => fun b => if b then [x∷σ] else [y∷τ]
+      | pat_shape_unit               => fun _ => [ctx]
+      | pat_shape_enum _             => fun _ => [ctx]
+      | pat_shape_bvec_split m n x y => fun _ => [x∷ty.bvec m; y∷ty.bvec n]
+      | pat_shape_bvec_exhaustive m  => fun _ => [ctx]
+      | pat_shape_union U x          => fun K => [x∷unionk_ty U K]
+      | pat_shape_tuple _ Δ _        => fun _ => Δ
+      | pat_shape_record _ Δ _       => fun _ => Δ
+      end%ctx.
+
+    (* Pattern match on a value. The result is a [PatternCase] that represents
+       the alternative corresponding to the value, together with an environment
+       that maps the variables of the pattern to values. *)
+    Definition newpattern_match_val {σ} (pat : PatternShape σ) :
+      Val σ -> { c : PatternCase pat & NamedEnv Val (PatternCaseCtx c) } :=
+      match pat with
+       | pat_shape_bool       =>
+           fun b => (b; [env])
+       | pat_shape_list σ x y =>
+           fun v : Val (ty.list σ) =>
+           match v with
+           | nil       => (true; [env])
+           | cons v vs => (false; [env].[x∷σ ↦ v].[y∷ty.list σ ↦ vs])
+           end
+       | pat_shape_prod σ τ x y =>
+           fun '(a, b) => (tt; [env].[x∷σ ↦ a].[y∷τ ↦ b])
+       | pat_shape_sum σ τ x y =>
+           fun v =>
+             match v with
+             | inl a => (true; [env].[x∷σ ↦ a])
+             | inr b => (false; [env].[y∷τ ↦ b])
+             end
+       | pat_shape_unit =>
+           fun _ => (tt; [env])
+       | pat_shape_enum E =>
+           fun v : enumt E => (v; [env])
+       | pat_shape_bvec_split m n x y =>
+           fun v =>
+             match bv.appView m n v with
+             | bv.isapp xs ys =>
+                 (tt; [env].[x∷ty.bvec m ↦ xs].[y∷ty.bvec n ↦ ys])
+             end
+       | pat_shape_bvec_exhaustive m =>
+           fun v => (v; [env])
+       | pat_shape_tuple σs Δ p =>
+           fun v => (tt; tuple_pattern_match_val p v)
+       | pat_shape_union U x =>
+           fun v => let (K, u) := unionv_unfold U v in (K; [env].[x∷unionk_ty U K ↦ u])
+       | pat_shape_record R Δ p =>
+           fun v => (tt; record_pattern_match_val p v)
+       end.
+
+    (* Reverse a pattern match. Given a [PatternCase] and an environment with
+       values for all variables in the pattern, reconstruct a value. *)
+    Definition newpattern_match_val_reverse {σ} (pat : PatternShape σ) :
+      forall (c : PatternCase pat), NamedEnv Val (PatternCaseCtx c) -> Val σ :=
+      match pat with
+      | pat_shape_bool       => fun b _ => b
+      | pat_shape_list σ x y =>
+          fun b =>
+            match b with
+            | true  => fun _ => nil
+            | false => fun Eht =>
+                         let (Eh,t) := env.snocView Eht in
+                         let (E,h)  := env.snocView Eh in
+                         cons h t
+            end
+      | pat_shape_prod σ τ x y =>
+          fun _ Exy =>
+            let (Ex,vy) := env.snocView Exy in
+            let (E,vx)  := env.snocView Ex in
+            (vx,vy)
+      | pat_shape_sum σ τ x y =>
+          fun b =>
+            match b with
+            | true  => fun vs => inl (env.head vs)
+            | false => fun vs => inr (env.head vs)
+            end
+      | pat_shape_unit =>
+          fun _ _ => tt
+      | pat_shape_enum E =>
+          fun v _ => v
+      | pat_shape_bvec_split m n x y =>
+          fun _ Exy =>
+            let (Ex,vy) := env.snocView Exy in
+            let (E,vx)  := env.snocView Ex in
+            bv.app vx vy
+      | pat_shape_bvec_exhaustive m =>
+          fun v _ => v
+      | pat_shape_tuple σs Δ p =>
+          fun _ vs => envrec.of_env (tuple_pattern_match_env_reverse p vs)
+      | pat_shape_union U x =>
+          fun K vs => unionv_fold U (K; env.head vs)
+      | pat_shape_record R Δ p =>
+          fun _ vs => recordv_fold R (record_pattern_match_env_reverse p vs)
+      end.
+
+    Definition newpattern_match_val_reverse' {σ} (pat : PatternShape σ) :
+      { c : PatternCase pat & NamedEnv Val (PatternCaseCtx c) } -> Val σ :=
+        fun c => newpattern_match_val_reverse pat (projT1 c) (projT2 c).
+
+    Lemma newpattern_match_val_inverse_right' {σ} (pat : PatternShape σ) :
+      forall (c : { pc : PatternCase pat & NamedEnv Val (PatternCaseCtx pc)}),
+        newpattern_match_val pat (newpattern_match_val_reverse' pat c) = c.
+    Proof.
+      destruct pat; cbn; intros [pc vs]; try progress cbn.
+      - env.destroy vs. reflexivity.
+      - destruct pc; now env.destroy vs.
+      - destruct pc; now env.destroy vs.
+      - destruct pc; now env.destroy vs.
+      - destruct pc; now env.destroy vs.
+      - now env.destroy vs.
+      - destruct pc; env.destroy vs.
+        now rewrite bv.appView_app.
+      - now env.destroy vs.
+      - destruct pc.
+        unfold tuple_pattern_match_val.
+        rewrite envrec.to_of_env.
+        now rewrite tuple_pattern_match_env_inverse_right.
+      - rewrite unionv_unfold_fold.
+        now env.destroy vs.
+      - destruct pc.
+        unfold record_pattern_match_val.
+        rewrite recordv_unfold_fold.
+        now rewrite record_pattern_match_env_inverse_right.
+    Qed.
+
+    Lemma newpattern_match_val_inverse_right {σ} (pat : PatternShape σ)
+      (pc : PatternCase pat) (δpc : NamedEnv Val (PatternCaseCtx pc)) :
+      newpattern_match_val pat (newpattern_match_val_reverse pat pc δpc) = (pc; δpc).
+    Proof. apply (newpattern_match_val_inverse_right' pat (pc;δpc)). Qed.
+
+    Lemma newpattern_match_val_inverse_left {σ} (pat : PatternShape σ) :
+      forall v : Val σ,
+        newpattern_match_val_reverse' pat (newpattern_match_val pat v) = v.
+    Proof.
+      destruct pat; cbn; intros v; try progress cbn.
+      - reflexivity.
+      - destruct v; reflexivity.
+      - destruct v; reflexivity.
+      - destruct v; reflexivity.
+      - destruct v; reflexivity.
+      - reflexivity.
+      - destruct bv.appView; reflexivity.
+      - reflexivity.
+      - unfold tuple_pattern_match_val.
+        rewrite tuple_pattern_match_env_inverse_left.
+        now rewrite envrec.of_to_env.
+      - destruct unionv_unfold as [K v'] eqn:?. cbn.
+        now rewrite <- Heqs, unionv_fold_unfold.
+      - unfold record_pattern_match_val.
+        rewrite record_pattern_match_env_inverse_left.
+        now rewrite recordv_fold_unfold.
     Qed.
 
   End Patterns.
